Change action unicode symbol

theories/Nominal.v
@@ -10,7 +10,7 @@ Section Nominal.
   Class Nominal `{Spt: Support X}: Prop := {
     nperm :> Perm X;
     support_spec : ∀ (x: X) (a b: name),
-      a ∉ (support x) → b ∉ (support x) → ⟨a,b⟩ • x ≡@{X} x
+      a ∉ (support x) → b ∉ (support x) → ⟨a,b⟩ ∙ x ≡@{X} x
 }.
 End Nominal.
 Arguments support_spec {_ PrA _ _ Nmn} : rename.
@@ -20,7 +20,7 @@ Arguments support_spec {_ PrA _ _ Nmn} : rename.
   
   Lemma lala : (a ∉ support x) → (c ∉ support x) →
     a ≠ b → b ≠ c →
-    ⟨ c, a ⟩ • ⟨ a, b ⟩ • x ≡ ⟨ c, b ⟩ • x.
+    ⟨ c, a ⟩ ∙ ⟨ a, b ⟩ ∙ x ≡ ⟨ c, b ⟩ ∙ x.
   Proof.
     intros; rewrite (perm_expand c a b).
     + repeat rewrite <- gact_compat. rewrite (support_spec x c a). auto.
